Mise à jour du modèle terminée. Ne reste que les preuves dans Convergence/Gathering.

current-formalism/Spectra/MultisetSpectrum.v
@@ -8,17 +8,15 @@
 (**************************************************************************)
 
 
-(* TODO: perform a correct installation of Containers *)
-Add LoadPath "~/.opam/coq-8.5/lib/coq/user-contrib/Containers" as Containers.
-Require Import Containers.MapInterface.
 Require Import Utf8_core.
 Require Import Arith_base.
 Require Import Omega.
 Require Import SetoidList.
-Require Import MMultisetInterface.
-Require Import MMultisetFacts.
-Require Import MMultisetExtraOps.
-(* Require MMultisetWMap. *)
+Require Import Pactole.Util.FMaps.FMapList.
+Require Import Pactole.Util.MMultiset.MMultisetWMap.
+Require Export Pactole.Util.MMultiset.MMultisetInterface.
+Require Import Pactole.Util.MMultiset.MMultisetFacts.
+Require Import Pactole.Util.MMultiset.MMultisetExtraOps.
 Require Import SetoidDec.
 Require Import Pactole.Util.Preliminary.
 Require Import Pactole.Setting.
@@ -26,29 +24,19 @@ Require Import Pactole.Setting.
 
 Close Scope R_scope.
 Set Implicit Arguments.
+Set Default Proof Using "All".
 Existing Instance multiplicity_compat.
 
-
-Print FMap.
 
 Section MultisetSpectrum.
 
 Context {loc : Type}.
 Context {loc_Setoid : Setoid loc}.
 Context {loc_EqDec : EqDec loc_Setoid}.
-Print OrderedType.
-Context {loc_EqDec : EqDec loc_Setoid}.
 Context {loc_RMS : RealMetricSpace loc}.
 Context {RobotsDef : NamesDef}.
 Context {Robots : Names}.
 
-
-(*
-Notation "m1  ≡  m2" := (Spect.eq m1 m2) (at level 70).
-Notation "m1  ⊆  m2" := (Spect.Subset m1 m2) (at level 70).
-Notation "m1  ==  m2" := (Spect.eq m1 m2) (at level 70, only parsing).
-Notation "m1  [c=]  m2" := (Spect.Subset m1 m2) (at level 70, only parsing).
-*)
 Lemma eq_refl_left : forall (e : loc) A (a b:A), (if equiv_dec e e then a else b) = a.
 Proof.
 intros e A a b.
@@ -60,24 +48,24 @@ Qed.
 
 (** **  Building multisets from lists  **)
 
-Definition multiset l := from_elements (List.map (fun x => (x, 1)) l).
+Definition make_multiset l := from_elements (List.map (fun x => (x, 1)) l).
 
-Lemma multiset_nil : multiset nil == empty.
+Lemma make_multiset_nil : make_multiset nil == empty.
 Proof. reflexivity. Qed.
 
-Lemma multiset_cons : forall x l, multiset (x :: l) == MMultisetInterface.add x 1 (multiset l).
+Lemma make_multiset_cons : forall x l, make_multiset (x :: l) == MMultisetInterface.add x 1 (make_multiset l).
 Proof. reflexivity. Qed.
 
-Lemma multiset_empty : forall l, multiset l == empty <-> l = nil.
+Lemma make_multiset_empty : forall l, make_multiset l == empty <-> l = nil.
 Proof.
-intro l. unfold multiset. rewrite from_elements_empty.
+intro l. unfold make_multiset. rewrite from_elements_empty.
 destruct l; cbn.
 - intuition.
 - split; intro Hl; inv Hl. discriminate.
 Qed.
 
-Lemma multiset_app : forall l l', multiset (l ++ l') == union (multiset l) (multiset l').
-Proof. intros. unfold multiset. now rewrite List.map_app, from_elements_append. Qed.
+Lemma make_multiset_app : forall l l', make_multiset (l ++ l') == union (make_multiset l) (make_multiset l').
+Proof. intros. unfold make_multiset. now rewrite List.map_app, from_elements_append. Qed.
 
 Lemma nequiv_sym: forall x y, ~x == y -> ~y == x.
 Proof.
@@ -87,19 +75,19 @@ Proof.
   contradiction.
 Qed.
 
-Instance multiset_compat : Proper (PermutationA equiv ==> equiv) multiset.
+Instance make_multiset_compat : Proper (PermutationA equiv ==> equiv) make_multiset.
 Proof.
-intros ? ? ?. unfold multiset. f_equiv. eapply PermutationA_map; eauto.
+intros ? ? ?. unfold make_multiset. f_equiv. eapply PermutationA_map; eauto.
 - autoclass.
 - repeat intro. split; hnf; auto.
 Qed.
 
-Lemma multiset_PermutationA : forall x l n, (multiset l)[x] = n ->
+Lemma make_multiset_PermutationA : forall x l n, (make_multiset l)[x] = n ->
   exists l', ~InA equiv x l' /\ PermutationA equiv l (alls x n ++ l').
 Proof.
 intros x l. induction l; intros n Hin.
-  exists nil. split. now auto. rewrite multiset_nil, empty_spec in Hin. subst n. simpl. reflexivity.
-  rewrite multiset_cons in Hin. destruct (equiv_dec x a) as [Heq | Heq].
+  exists nil. split. now auto. rewrite make_multiset_nil, empty_spec in Hin. subst n. simpl. reflexivity.
+  rewrite make_multiset_cons in Hin. destruct (equiv_dec x a) as [Heq | Heq].
   - setoid_rewrite <- Heq. rewrite <- Heq in Hin. rewrite add_spec in Hin. destruct n.
     + rewrite eq_refl_left in Hin.
       omega.
@@ -111,11 +99,11 @@ intros x l. induction l; intros n Hin.
     transitivity (a :: alls x n ++ l'); now constructor || apply (PermutationA_middle _).
 Qed.
 
-Lemma multiset_alls : forall x n, multiset (alls x n) == singleton x n.
+Lemma make_multiset_alls : forall x n, make_multiset (alls x n) == singleton x n.
 Proof.
 intros x n. induction n.
-+ now rewrite singleton_0, multiset_nil.
-+ simpl alls. rewrite multiset_cons. rewrite IHn. intro y. rewrite singleton_spec.
++ now rewrite singleton_0, make_multiset_nil.
++ simpl alls. rewrite make_multiset_cons. rewrite IHn. intro y. rewrite singleton_spec.
   destruct (equiv_dec y x) as [Heq | Heq].
   - rewrite Heq, add_spec, singleton_spec.
     destruct (equiv_dec x x) as [_ | Helim]. omega. now elim Helim.
@@ -123,9 +111,9 @@ intros x n. induction n.
     destruct (equiv_dec y x); trivial; []. contradiction.
 Qed.
 
-Corollary multiset_In : forall x l, In x (multiset l) <-> InA equiv x l.
+Corollary make_multiset_In : forall x l, In x (make_multiset l) <-> InA equiv x l.
 Proof.
-intros x l. unfold multiset. rewrite from_elements_In.
+intros x l. unfold make_multiset. rewrite from_elements_In.
 setoid_rewrite InA_map_iff; autoclass.
 + split; intro Hin.
   - destruct Hin as [n [[y [[Heq _] Hy]] Hn]]. hnf in *. cbn in *. now rewrite <- Heq.
@@ -133,88 +121,95 @@ setoid_rewrite InA_map_iff; autoclass.
 + intros ? ? Heq. now split.
 Qed.
 
-Theorem multiset_map : forall f, Proper (equiv ==> equiv) f ->
-  forall l, multiset (List.map f l) == map f (multiset l).
-Proof. intros. unfold multiset. now rewrite map_from_elements, map_map, map_map. Qed.
+Theorem make_multiset_map : forall f, Proper (equiv ==> equiv) f ->
+  forall l, make_multiset (List.map f l) == map f (make_multiset l).
+Proof. intros. unfold make_multiset. now rewrite map_from_elements, map_map, map_map. Qed.
 
-Theorem multiset_filter : forall f, Proper (equiv ==> Logic.eq) f ->
-  forall l, multiset (List.filter f l) == filter f (multiset l).
+Theorem make_multiset_filter : forall f, Proper (equiv ==> Logic.eq) f ->
+  forall l, make_multiset (List.filter f l) == filter f (make_multiset l).
 Proof.
 intros f Hf l. induction l as [| e l].
-+ intro. rewrite (filter_compat Hf), multiset_nil; try apply multiset_nil; [].
++ intro. rewrite (filter_compat Hf), make_multiset_nil; try apply make_multiset_nil; [].
   now rewrite filter_empty.
 + simpl List.filter. destruct (f e) eqn:Htest.
-  - do 2 rewrite multiset_cons. rewrite filter_add, Htest, IHl; trivial; reflexivity || omega.
-  - rewrite multiset_cons, filter_add, Htest, IHl; trivial; reflexivity || omega.
+  - do 2 rewrite make_multiset_cons. rewrite filter_add, Htest, IHl; trivial; reflexivity || omega.
+  - rewrite make_multiset_cons, filter_add, Htest, IHl; trivial; reflexivity || omega.
 Qed.
 
-Theorem cardinal_multiset : forall l, cardinal (multiset l) = length l.
+Theorem cardinal_make_multiset : forall l, cardinal (make_multiset l) = length l.
 Proof.
-induction l; simpl.
-+ now rewrite multiset_nil, cardinal_empty.
-+ rewrite multiset_cons, cardinal_add. apply f_equal, IHl.
+induction l.
++ now rewrite make_multiset_nil, cardinal_empty.
++ rewrite make_multiset_cons, cardinal_add. simpl. apply f_equal, IHl.
 Qed.
 
-Theorem multiset_spec : forall x l, (multiset l)[x] = countA_occ _ equiv_dec x l.
+Theorem make_multiset_spec : forall x l, (make_multiset l)[x] = countA_occ _ equiv_dec x l.
 Proof.
-intros x l. induction l; simpl.
-+ rewrite multiset_nil. now apply empty_spec.
-+ rewrite multiset_cons. destruct (equiv_dec a x) as [Heq | Hneq].
-  - rewrite Heq. rewrite add_spec. rewrite IHl.
-    rewrite eq_refl_left.
-    omega.
+intros x l. induction l.
++ rewrite make_multiset_nil. now rewrite empty_spec.
++ rewrite make_multiset_cons. simpl countA_occ. destruct (equiv_dec a x) as [Heq | Hneq].
+  - rewrite <- Heq at 1. rewrite add_spec, eq_refl_left, Heq, IHl. omega.
   - apply nequiv_sym in Hneq. rewrite add_other. now apply IHl. assumption.
 Qed.
 
-Lemma multiset_remove : forall x l,
-  multiset (removeA equiv_dec x l) == remove x (multiset l)[x] (multiset l).
+Lemma make_multiset_remove : forall x l,
+  make_multiset (removeA equiv_dec x l) == remove x (make_multiset l)[x] (make_multiset l).
 Proof.
-intros x l y. induction l as [| a l]; simpl.
-* rewrite multiset_nil. do 2 rewrite empty_spec. now rewrite remove_0, empty_spec.
-* rewrite multiset_cons. destruct (equiv_dec y x) as [Hyx | Hyx], (equiv_dec x a) as [Hxa | Hxa].
+intros x l y. induction l as [| a l].
+* rewrite make_multiset_nil. rewrite empty_spec. now rewrite remove_0, empty_spec.
+* rewrite make_multiset_cons. simpl removeA.
+  destruct (equiv_dec y x) as [Hyx | Hyx], (equiv_dec x a) as [Hxa | Hxa].
   + rewrite Hyx, Hxa in *. rewrite IHl. setoid_rewrite remove_same. rewrite Hxa, add_same. omega.
-  + rewrite Hyx in *. rewrite multiset_cons, add_other; auto.
+  + rewrite Hyx in *. rewrite make_multiset_cons, add_other; auto.
     rewrite IHl. do 2 rewrite remove_same. omega.
   + rewrite IHl. repeat rewrite remove_other; auto; [].
     rewrite Hxa in *. rewrite add_other; auto.
-  + rewrite multiset_cons. rewrite remove_other; auto. destruct (equiv_dec y a) as [Hya | Hya].
+  + rewrite make_multiset_cons. rewrite remove_other; auto. destruct (equiv_dec y a) as [Hya | Hya].
     - rewrite Hya in *. do 2 rewrite add_same. rewrite IHl. now rewrite remove_other.
     - repeat rewrite add_other; trivial. rewrite IHl. rewrite remove_other; auto.
 Qed.
 
-Lemma multiset_support : forall x l, InA equiv x (support (multiset l)) <-> InA equiv x l.
+Lemma make_multiset_support : forall x l, InA equiv x (support (make_multiset l)) <-> InA equiv x l.
 Proof.
-intros x l. rewrite support_spec. unfold In.
-rewrite multiset_spec. apply countA_occ_pos. autoclass.
+intros x l. Locate support_spec. rewrite support_spec. unfold In.
+rewrite make_multiset_spec. apply countA_occ_pos. autoclass.
 Qed.
 
 (** Building a spectrum from a configuration *)
 
-Instance multiset_spectrum : Spectrum loc := {|
-  spectrum := t;
+Global Instance multiset_spectrum : Spectrum loc := {|
+  spectrum := multiset;
   spectrum_Setoid := MMultiset_Setoid;
   spectrum_EqDec := MMultisetEqDec;
   
-  spect_from_config conf := multiset (config_list conf);
+  spect_from_config conf := make_multiset (config_list conf);
   spect_is_ok s conf := forall l, s[l] = countA_occ _ equiv_dec l (config_list conf) |}.
-Proof.
+(* BUG? proof is forbidden now *)
+(* Proof. *)
 + intros conf1 conf2 Hconf x. unfold spect_from_config. do 2 f_equiv.
   apply eqlistA_PermutationA_subrelation. apply config_list_compat. assumption.
-+ unfold spect_from_config, spect_is_ok. intros. apply multiset_spec.
++ unfold spect_from_config, spect_is_ok. intros. apply make_multiset_spec.
 Defined.
+
 
 Lemma spect_from_config_map  : forall f, Proper (equiv ==> equiv) f ->
   forall config : configuration,
   @equiv spectrum spectrum_Setoid (map f (spect_from_config config)) (spect_from_config (map_config f config)).
-Proof. repeat intro. unfold spect_from_config. cbn. now rewrite config_list_map, multiset_map. Qed.
+Proof.
+repeat intro. unfold spect_from_config, multiset_spectrum.
+now rewrite config_list_map, make_multiset_map.
+Qed.
 
 Theorem cardinal_spect_from_config : forall conf, cardinal (spect_from_config conf) = nG + nB.
-Proof. intro. unfold spect_from_config. cbn. now rewrite cardinal_multiset, config_list_length. Qed.
+Proof.
+intro. unfold spect_from_config, multiset_spectrum.
+now rewrite cardinal_make_multiset, config_list_length.
+Qed.
 
 Property pos_in_config : forall conf id, In (conf id) (spect_from_config conf).
 Proof.
 intros conf id. cbn. unfold In.
-rewrite multiset_spec. rewrite (countA_occ_pos _).
+rewrite make_multiset_spec. rewrite (countA_occ_pos _).
 rewrite config_list_InA. now exists id.
 Qed.
 
@@ -222,7 +217,8 @@ Property spect_from_config_In : forall config l,
   In l (spect_from_config config) <-> exists id, equiv (config id) l.
 Proof.
 intros config l. split; intro Hin.
-+ assert (Heq := spect_from_config_spec config). cbn in Heq, Hin.
++ assert (Heq := spect_from_config_spec config).
+  unfold spect_is_ok, spect_from_config, multiset_spectrum in *.
   unfold In in Hin. rewrite Heq, (countA_occ_pos _), config_list_spec in Hin.
   rewrite (InA_map_iff _ _) in Hin.
   - firstorder.
@@ -232,4 +228,4 @@ Qed.
 
 End MultisetSpectrum.
 
-Global Notation "s [ x ]" := (multiplicity x s) (at level 2, no associativity, format "s [ x ]").
+Global Notation "s [ x ]" := (multiplicity x (s : spectrum)) (at level 2, no associativity, format "s [ x ]").
