current-formalism/Spaces/R2.v
@@ -1921,7 +1921,8 @@ destruct (Exists_dec (fun x => x <> pt1 /\ on_circle (SEC (pt1 :: l)) x = true))
     ++ unfold d, r, c. rewrite dist_sym. apply SEC_spec1. now right.
     ++ intro. do 2 subst. apply Hsmall. rewrite Exists_exists. exists pt2. repeat split.
        -- now right.
-       -- clear -Hon1 Hnodup Hin2. unfold pt2. apply farthest_from_in_except_diff. intro Heq. subst.
+       -- clear -Hon1 Hnodup Hin2. unfold pt2. apply farthest_from_in_except_diff. intro Heq. subst c.
+          (* BUG? subst without c does not work! *)
           rewrite <- Heq in Hon1 at 2. rewrite center_on_circle, SEC_zero_radius_incl_singleton in Hon1.
           destruct Hon1 as [pt Hincl].
           assert (pt = pt1). { specialize (Hincl pt1 ltac:(intuition)). simpl in Hincl. intuition. }
